Semantic/ModalCapybara/Syntax/Ty.lean
@@ -40,6 +40,7 @@ def Ty.rename : Ty sort s1 -> Rename s1 s2 -> Ty sort s2
 | .arrow T1 cs T2, f => .arrow (T1.rename f) (cs.rename f) (T2.rename (f.lift))
 | .poly T1 cs T2, f => .poly (T1.rename f) (cs.rename f) (T2.rename (f.lift))
 | .cpoly m cs T, f => .cpoly m (cs.rename f) (T.rename (f.lift))
+| .modal Ψ T, f => .modal (Ψ.rename f) (T.rename f)
 | .unit, _ => .unit
 | .cap cs, f => .cap (cs.rename f)
 | .bool, _ => .bool
@@ -56,6 +57,7 @@ def Ty.rename_id {T : Ty sort s} : T.rename (Rename.id) = T := by
   case arrow ih1 ih2 => simp [Ty.rename, Rename.lift_id, CaptureSet.rename_id, ih1, ih2]
   case poly ih1 ih2 => simp [Ty.rename, Rename.lift_id, CaptureSet.rename_id, ih1, ih2]
   case cpoly ih => simp [Ty.rename, Rename.lift_id, CaptureSet.rename_id, ih]
+  case modal ih => simp [Ty.rename, SepCtx.rename_id, ih]
   case unit => rfl
   case cap => simp [Ty.rename, CaptureSet.rename_id]
   case bool => rfl
@@ -73,6 +75,7 @@ theorem Ty.rename_comp {T : Ty sort s1} {f : Rename s1 s2} {g : Rename s2 s3} :
   case arrow ih1 ih2 => simp [Ty.rename, Rename.lift_comp, CaptureSet.rename_comp, ih1, ih2]
   case poly ih1 ih2 => simp [Ty.rename, Rename.lift_comp, CaptureSet.rename_comp, ih1, ih2]
   case cpoly ih => simp [Ty.rename, Rename.lift_comp, CaptureSet.rename_comp, ih]
+  case modal ih => simp [Ty.rename, SepCtx.rename_comp, ih]
   case unit => rfl
   case cap => simp [Ty.rename, CaptureSet.rename_comp]
   case bool => rfl
@@ -93,6 +96,7 @@ def Ty.captureSet : Ty .capt s -> CaptureSet s
 | .arrow _ cs _ => cs
 | .poly _ cs _ => cs
 | .cpoly _ cs _ => cs
+| .modal _ _ => .empty
 | .cap cs => cs
 | .cell cs => cs
 | .reader cs => cs
@@ -105,6 +109,7 @@ def Ty.refineCaptureSet : Ty .capt s -> CaptureSet s -> Ty .capt s
 | .arrow T1 _ T2, cs => .arrow T1 cs T2
 | .poly T1 _ T2, cs => .poly T1 cs T2
 | .cpoly m _ T, cs => .cpoly m cs T
+| .modal Ψ T, _ => .modal Ψ T
 | .cap _, cs => .cap cs
 | .cell _, cs => .cell cs
 | .reader _, cs => .reader cs
@@ -120,6 +125,7 @@ inductive Ty.IsClosed : Ty sort s -> Prop where
 | poly : Ty.IsClosed T1 -> CaptureSet.IsClosed cs -> Ty.IsClosed T2 ->
     Ty.IsClosed (.poly T1 cs T2)
 | cpoly : CaptureSet.IsClosed cs -> Ty.IsClosed T -> Ty.IsClosed (.cpoly m cs T)
+| modal : SepCtx.IsClosed Ψ -> Ty.IsClosed T -> Ty.IsClosed (.modal Ψ T)
 | unit : Ty.IsClosed .unit
 | cap : CaptureSet.IsClosed cs -> Ty.IsClosed (.cap cs)
 | bool : Ty.IsClosed .bool
